Extraction.lean
@@ -2,11 +2,26 @@
 -- Import modules here that should be built as part of the library.
 import Extraction.Basic
 
-#show_sketch (1 : Nat) + (2 |ₛ [3]ₛ)
-
 opaque P : Nat → Nat → Nat → Prop
 opaque Q : Prop
-opaque R : Nat → Prop
 
-example (h : P 1 2 3 ↔ Q) (h2 : P 1 2 3 ↔ R 1) : P 1 2 3 := by
+/-- error: unknown free variable `_fvar.177` -/
+#guard_msgs in
+example (h : P 1 2 3 ↔ Q) : P 1 2 3 := by
+  grind extract min_ast
+
+/--
+error: unsolved goals
+⊢ P 1 2 3
+-/
+#guard_msgs in
+theorem b : P 1 2 3 := by
+  grind extract min_ast
+
+/--
+error: unsolved goals
+⊢ [true] ++ [] = [false]
+-/
+#guard_msgs in
+theorem a : [true] ++ [] = [false] := by
   grind extract min_ast
